subprogram theory
Start some development about extending programs. In particular it is
proven that if we extend a program with a suitable block, the
BST_JumpOutside status code disappears.

src/core-props/bir_program_valid_stateScript.sml
@@ -3,7 +3,6 @@ open bir_auxiliaryTheory
 open bir_envTheory bir_valuesTheory
 open bir_programTheory HolBACoreSimps;
 
-
 val _ = new_theory "bir_program_valid_state";
 
 
@@ -14,8 +13,10 @@ val _ = new_theory "bir_program_valid_state";
 val bir_is_valid_labels_def = Define `bir_is_valid_labels p =
   ALL_DISTINCT (bir_labels_of_program p)`;
 
+val bir_program_is_empty_def = Define `bir_program_is_empty (BirProgram p) <=> NULL p`
+
 val bir_is_valid_program_def = Define `bir_is_valid_program p <=>
-   (bir_is_valid_labels p) /\ ~(p = BirProgram [])`;
+   (bir_is_valid_labels p) /\ ~(bir_program_is_empty p)`;
 
 
 (* This allows some nice rewrites *)
@@ -150,7 +151,8 @@ val bir_pc_first_valid = store_thm ("bir_pc_first_valid",
 Cases >> rename1 `BirProgram p` >>
 SIMP_TAC std_ss [bir_pc_first_def, bir_is_valid_pc_block_pc] >>
 Cases_on `p` >> (
-  SIMP_TAC list_ss [bir_is_valid_program_def, bir_labels_of_program_def]
+  SIMP_TAC list_ss [bir_is_valid_program_def, bir_labels_of_program_def,
+    bir_program_is_empty_def]
 ));
 
 
@@ -182,18 +184,25 @@ val bir_state_init_valid = store_thm ("bir_state_init_valid",
 SIMP_TAC (std_ss++holBACore_ss++holBACore_ss) [bir_is_valid_state_def, bir_state_init_def,
   bir_pc_first_valid, bir_is_well_typed_env_empty]);
 
+
+val bir_exec_step_invalid_pc_THM = store_thm ("bir_exec_step_invalid_pc_THM",
+ ``!p st. ~(bir_is_valid_pc p st.bst_pc) ==>
+          (bir_exec_step p st = (NONE, if (bir_state_is_terminated st) then st else bir_state_set_failed st))``,
+
+METIS_TAC[bir_exec_step_def, bir_get_current_statement_IS_SOME, optionTheory.option_CLAUSES]);
+
+
 (* valid states allow some nice rewrite for bir_exec_step *)
 val bir_exec_step_valid_THM = store_thm ("bir_exec_step_valid_THM",
- ``!p st. bir_is_valid_state p st ==>
+ ``!p st. bir_is_valid_pc p st.bst_pc ==>
           (if bir_state_is_terminated st then
              (bir_exec_step p st = (NONE, st))
            else
-             (bir_is_valid_pc p st.bst_pc) /\
              (?stmt. (bir_get_current_statement p st.bst_pc = SOME stmt) /\
                      (bir_exec_step p st = (bir_exec_stmt p stmt st))))``,
 
 REPEAT STRIP_TAC >>
-FULL_SIMP_TAC std_ss [bir_exec_step_def, bir_is_valid_state_def] >>
+FULL_SIMP_TAC std_ss [bir_exec_step_def] >>
 Cases_on `bir_state_is_terminated st` >> ASM_SIMP_TAC (std_ss++boolSimps.CONJ_ss) [] >>
 `IS_SOME (bir_get_current_statement p st.bst_pc)` suffices_by METIS_TAC[optionTheory.IS_SOME_EXISTS] >>
 FULL_SIMP_TAC std_ss [bir_get_current_statement_IS_SOME,
@@ -201,11 +210,10 @@ FULL_SIMP_TAC std_ss [bir_get_current_statement_IS_SOME,
 
 
 val bir_exec_step_state_valid_THM = store_thm ("bir_exec_step_state_valid_THM",
- ``!p st. bir_is_valid_state p st ==>
+ ``!p st. bir_is_valid_pc p st.bst_pc ==>
           (if bir_state_is_terminated st then
              (bir_exec_step_state p st = st)
            else
-             (bir_is_valid_pc p st.bst_pc) /\
              (?stmt. (bir_get_current_statement p st.bst_pc = SOME stmt) /\
                      (bir_exec_step_state p st = (bir_exec_stmt_state p stmt st))))``,
 
@@ -219,21 +227,14 @@ METIS_TAC [pairTheory.SND]);
    bir_is_valid_state is an invariant
    ------------------------------------------------------------------------- *)
 
-val bir_is_valid_state_set_failed = prove (
-  ``!p st. bir_is_valid_state p st ==>
-           bir_is_valid_state p (bir_state_set_failed st)``,
-SIMP_TAC (std_ss++holBACore_ss++holBACore_ss) [bir_is_valid_state_def, bir_state_set_failed_def]);
+val bir_exec_stmtB_well_typed_env_declare = prove (
+  ``!st v ty. bir_is_well_typed_env st.bst_environ ==>
+              bir_is_well_typed_env (bir_exec_stmt_declare v ty st).bst_environ``,
 
-
-val bir_exec_stmtB_valid_state_invar_declare = prove (
-  ``!p st v ty. bir_is_valid_state p st ==>
-                bir_is_valid_state p (bir_exec_stmt_declare v ty st)``,
-
-SIMP_TAC (std_ss++boolSimps.LIFT_COND_ss) [bir_exec_stmt_declare_def, LET_THM,
-  bir_is_valid_state_set_failed, bir_var_type_def, bir_var_name_def] >>
-REPEAT STRIP_TAC >>
+SIMP_TAC (std_ss++bir_TYPES_ss++boolSimps.LIFT_COND_ss) [bir_exec_stmt_declare_def, LET_THM,
+  bir_var_type_def, bir_var_name_def, bir_state_set_failed_def] >>
 Cases_on `bir_env_varname_is_bound st.bst_environ v` >> ASM_REWRITE_TAC[] >>
-
+REPEAT STRIP_TAC >>
 `?env. (bir_env_update v (bir_declare_initial_value ty) ty st.bst_environ = SOME env)` by (
   Cases_on `st.bst_environ` >>
   Cases_on `ty` >> (
@@ -244,67 +245,67 @@ FULL_SIMP_TAC (std_ss++holBACore_ss) [bir_is_valid_state_def] >>
 METIS_TAC[bir_env_update_is_well_typed_env]);
 
 
-val bir_exec_stmtB_valid_state_invar_assign = prove (
-  ``!p st v ex. bir_is_valid_state p st ==>
-                bir_is_valid_state p (bir_exec_stmt_assign v ex st)``,
+val bir_exec_stmtB_well_typed_env_assign = prove (
+  ``!st v ex. bir_is_well_typed_env st.bst_environ ==>
+              bir_is_well_typed_env (bir_exec_stmt_assign v ex st).bst_environ``,
 Cases_on `v` >> rename1 `BVar v ty` >>
 REPEAT STRIP_TAC >>
 SIMP_TAC std_ss [bir_exec_stmt_assign_def, LET_THM] >>
 Cases_on `bir_env_write (BVar v ty) (bir_eval_exp ex st.bst_environ)
        st.bst_environ` >> (
-  ASM_SIMP_TAC std_ss [bir_is_valid_state_set_failed]
+  ASM_SIMP_TAC (std_ss++bir_TYPES_ss) [bir_state_set_failed_def]
 ) >>
 FULL_SIMP_TAC (std_ss++holBACore_ss) [bir_is_valid_state_def] >>
 METIS_TAC[bir_env_write_is_well_typed_env]);
 
 
-val bir_exec_stmtB_valid_state_invar_assert = prove (
-  ``!p st ex. bir_is_valid_state p st ==>
-              bir_is_valid_state p (bir_exec_stmt_assert ex st)``,
+val bir_exec_stmtB_well_typed_env_assert = prove (
+  ``!st ex. bir_is_well_typed_env st.bst_environ ==>
+            bir_is_well_typed_env (bir_exec_stmt_assert ex st).bst_environ``,
 
 SIMP_TAC (std_ss++holBACore_ss) [bir_exec_stmt_assert_def] >>
 REPEAT GEN_TAC >> STRIP_TAC >>
 REPEAT CASE_TAC >> (
-  ASM_SIMP_TAC std_ss [bir_is_valid_state_set_failed]
+  ASM_SIMP_TAC (std_ss++bir_TYPES_ss) [bir_state_set_failed_def]
 ));
 
 
-val bir_exec_stmtB_valid_state_invar_assume = prove (
-  ``!p st ex. bir_is_valid_state p st ==>
-              bir_is_valid_state p (bir_exec_stmt_assume ex st)``,
+val bir_exec_stmtB_well_typed_env_assume = prove (
+  ``!st ex. bir_is_well_typed_env st.bst_environ ==>
+            bir_is_well_typed_env (bir_exec_stmt_assume ex st).bst_environ``,
 
 SIMP_TAC (std_ss++holBACore_ss) [bir_exec_stmt_assume_def] >>
 REPEAT GEN_TAC >> STRIP_TAC >>
 REPEAT CASE_TAC >> (
-  ASM_SIMP_TAC std_ss [bir_is_valid_state_set_failed]
+  ASM_SIMP_TAC (std_ss++bir_TYPES_ss) [bir_state_set_failed_def]
 ) >>
 FULL_SIMP_TAC (std_ss++holBACore_ss) [bir_is_valid_state_def]);
 
 
-val bir_exec_stmtB_valid_state_invar_observe = prove (
-  ``!p st ec.
-      bir_is_valid_state p st ==>
-      bir_is_valid_state p (bir_exec_stmt_observe_state ec st)``,
+val bir_exec_stmtB_well_typed_env_observe = prove (
+  ``!st ec.
+      bir_is_well_typed_env st.bst_environ ==>
+      bir_is_well_typed_env (bir_exec_stmt_observe_state ec st).bst_environ``,
 
 SIMP_TAC (std_ss++holBACore_ss) [bir_exec_stmt_observe_state_def] >>
 REPEAT GEN_TAC >> STRIP_TAC >>
 REPEAT CASE_TAC >> (
-  ASM_SIMP_TAC std_ss [bir_is_valid_state_set_failed]
+  ASM_SIMP_TAC (std_ss++bir_TYPES_ss) [bir_state_set_failed_def]
 ));
 
 
-val bir_exec_stmtB_valid_state_invar = store_thm ("bir_exec_stmtB_valid_state_invar",
-``!p st stmt. bir_is_valid_state p st ==>
-              bir_is_valid_state p (bir_exec_stmtB_state stmt st)``,
+val bir_exec_stmtB_well_typed_env = store_thm ("bir_exec_stmtB_well_typed_env",
+``!st stmt. bir_is_well_typed_env st.bst_environ ==>
+            bir_is_well_typed_env (bir_exec_stmtB_state stmt st).bst_environ``,
 
 REPEAT STRIP_TAC >>
 Cases_on `stmt` >> (
   ASM_SIMP_TAC std_ss [bir_exec_stmtB_state_REWRS,
-    bir_exec_stmtB_valid_state_invar_declare,
-    bir_exec_stmtB_valid_state_invar_assign,
-    bir_exec_stmtB_valid_state_invar_assume,
-    bir_exec_stmtB_valid_state_invar_assert,
-    bir_exec_stmtB_valid_state_invar_observe]
+    bir_exec_stmtB_well_typed_env_declare,
+    bir_exec_stmtB_well_typed_env_assign,
+    bir_exec_stmtB_well_typed_env_assume,
+    bir_exec_stmtB_well_typed_env_assert,
+    bir_exec_stmtB_well_typed_env_observe]
 ));
 
 
@@ -321,69 +322,143 @@ Cases_on `stmt` >> (
   FULL_SIMP_TAC (std_ss++holBACore_ss) [bir_state_set_failed_def]
 ));
 
+val bir_exec_stmtB_valid_state_invar = store_thm ("bir_exec_stmtB_valid_state_invar",
+``!p st stmt. bir_is_valid_state p st ==>
+              bir_is_valid_state p (bir_exec_stmtB_state stmt st)``,
 
-val bir_exec_stmt_jmp_to_label_valid_state_invar = store_thm ("bir_exec_stmt_jmp_to_label_valid_state_invar",
-  ``!p st l. bir_is_valid_state p st ==>
-             bir_is_valid_state p (bir_exec_stmt_jmp_to_label p l st)``,
+SIMP_TAC std_ss [bir_is_valid_state_def,
+  bir_exec_stmtB_pc_unchanged, bir_exec_stmtB_well_typed_env]);
+
+
+val bir_exec_stmt_jmp_to_label_valid_pc = store_thm ("bir_exec_stmt_jmp_to_label_valid_pc",
+  ``!p st l. bir_is_valid_pc p st.bst_pc ==>
+             bir_is_valid_pc p (bir_exec_stmt_jmp_to_label p l st).bst_pc``,
 SIMP_TAC std_ss [bir_exec_stmt_jmp_to_label_def] >>
 REPEAT STRIP_TAC >>
 COND_CASES_TAC >| [
-  FULL_SIMP_TAC (std_ss++holBACore_ss) [bir_is_valid_state_def,
-    bir_is_valid_pc_block_pc],
+  FULL_SIMP_TAC (std_ss++holBACore_ss) [bir_is_valid_pc_block_pc],
 
-  FULL_SIMP_TAC (std_ss++holBACore_ss) [bir_is_valid_state_def]
+  FULL_SIMP_TAC (std_ss++holBACore_ss) []
 ]);
 
 
-val bir_exec_stmt_jmp_valid_state_invar = store_thm ("bir_exec_stmt_jmp_valid_state_invar",
-  ``!p st l. bir_is_valid_state p st ==>
-             bir_is_valid_state p (bir_exec_stmt_jmp p l st)``,
+val bir_exec_stmt_jmp_valid_pc = store_thm ("bir_exec_stmt_jmp_valid_pc",
+  ``!p st l. bir_is_valid_pc p st.bst_pc ==>
+             bir_is_valid_pc p (bir_exec_stmt_jmp p l st).bst_pc``,
 SIMP_TAC std_ss [bir_exec_stmt_jmp_def] >>
 REPEAT STRIP_TAC >> CASE_TAC >> (
-  ASM_SIMP_TAC std_ss [bir_exec_stmt_jmp_to_label_valid_state_invar,
-                       bir_is_valid_state_set_failed]
+  ASM_SIMP_TAC (std_ss++bir_TYPES_ss) [
+     bir_exec_stmt_jmp_to_label_valid_pc,
+     bir_state_set_failed_def]
 ));
 
 
-val bir_exec_stmtE_valid_state_invar_jmp = prove (
-  ``!p st l. bir_is_valid_state p st ==>
-             bir_is_valid_state p (bir_exec_stmtE p (BStmt_Jmp l) st)``,
-SIMP_TAC std_ss [bir_exec_stmtE_def, bir_exec_stmt_jmp_valid_state_invar]);
+val bir_exec_stmtE_valid_pc_jmp = prove (
+  ``!p st l. bir_is_valid_pc p st.bst_pc ==>
+             bir_is_valid_pc p (bir_exec_stmtE p (BStmt_Jmp l) st).bst_pc``,
+SIMP_TAC std_ss [bir_exec_stmtE_def, bir_exec_stmt_jmp_valid_pc]);
 
 
-val bir_exec_stmtE_valid_state_invar_cjmp = prove (
+val bir_exec_stmtE_valid_pc_cjmp = prove (
   ``!p st ex l1 l2.
-       bir_is_valid_state p st ==>
-       bir_is_valid_state p (bir_exec_stmtE p (BStmt_CJmp ex l1 l2) st)``,
+       bir_is_valid_pc p st.bst_pc ==>
+       bir_is_valid_pc p (bir_exec_stmtE p (BStmt_CJmp ex l1 l2) st).bst_pc``,
 SIMP_TAC std_ss [bir_exec_stmtE_def, bir_exec_stmt_cjmp_def] >>
 REPEAT STRIP_TAC >>
 Cases_on `bir_dest_bool_val (bir_eval_exp ex st.bst_environ)` >- (
-  ASM_SIMP_TAC std_ss [bir_is_valid_state_set_failed]
+  ASM_SIMP_TAC (std_ss++bir_TYPES_ss) [bir_state_set_failed_def]
 ) >>
 rename1 `SOME c` >>
 Cases_on `c` >> (
-  ASM_SIMP_TAC std_ss [bir_exec_stmt_jmp_valid_state_invar]
+  ASM_SIMP_TAC std_ss [bir_exec_stmt_jmp_valid_pc]
 ));
 
 
-val bir_exec_stmtE_valid_state_invar_halt = prove (
-  ``!p st ex.  bir_is_valid_state p st ==>
-               bir_is_valid_state p (bir_exec_stmtE p (BStmt_Halt ex) st)``,
+val bir_exec_stmtE_valid_pc_halt = prove (
+  ``!p st ex.  bir_is_valid_pc p st.bst_pc ==>
+               bir_is_valid_pc p (bir_exec_stmtE p (BStmt_Halt ex) st).bst_pc``,
 
-SIMP_TAC (std_ss++holBACore_ss) [bir_exec_stmtE_def, bir_exec_stmt_halt_def,
-  bir_is_valid_state_def]);
+SIMP_TAC (std_ss++holBACore_ss) [bir_exec_stmtE_def, bir_exec_stmt_halt_def]);
+
+
+val bir_exec_stmtE_valid_pc = store_thm ("bir_exec_stmtE_valid_pc",
+``!p st stmt. bir_is_valid_pc p st.bst_pc ==>
+              bir_is_valid_pc p (bir_exec_stmtE p stmt st).bst_pc``,
+
+REPEAT STRIP_TAC >>
+Cases_on `stmt` >> (
+  ASM_SIMP_TAC std_ss [
+    bir_exec_stmtE_valid_pc_cjmp,
+    bir_exec_stmtE_valid_pc_jmp,
+    bir_exec_stmtE_valid_pc_halt]
+));
+
+
+val bir_exec_stmtE_env_unchanged = store_thm ("bir_exec_stmtE_env_unchanged",
+``!p st stmt. (bir_exec_stmtE p stmt st).bst_environ = st.bst_environ``,
+
+REPEAT STRIP_TAC >>
+Cases_on `stmt` >> (
+  SIMP_TAC std_ss [bir_exec_stmtE_def,
+    bir_exec_stmt_halt_def, bir_exec_stmt_jmp_def,
+    bir_exec_stmt_cjmp_def, bir_exec_stmt_jmp_to_label_def,
+    bir_state_set_failed_def] >>
+  REPEAT CASE_TAC >>
+  SIMP_TAC (std_ss++holBACore_ss) []
+));
 
 
 val bir_exec_stmtE_valid_state_invar = store_thm ("bir_exec_stmtE_valid_state_invar",
 ``!p st stmt. bir_is_valid_state p st ==>
               bir_is_valid_state p (bir_exec_stmtE p stmt st)``,
 
+SIMP_TAC std_ss [bir_is_valid_state_def,
+  bir_exec_stmtE_env_unchanged, bir_exec_stmtE_valid_pc]);
+
+
+
+
+val bir_exec_step_valid_pc = store_thm ("bir_exec_step_valid_pc",
+``!p st. bir_is_valid_pc p (bir_exec_step_state p st).bst_pc <=>
+         bir_is_valid_pc p st.bst_pc``,
+
 REPEAT STRIP_TAC >>
+Cases_on `bir_state_is_terminated st` >- (
+  FULL_SIMP_TAC std_ss [bir_exec_step_state_def, bir_exec_step_def]
+) >>
+EQ_TAC >> REPEAT STRIP_TAC >- (
+  CCONTR_TAC >>
+  FULL_SIMP_TAC std_ss [bir_exec_step_invalid_pc_THM, bir_exec_step_state_def] >>
+  REV_FULL_SIMP_TAC (std_ss++bir_TYPES_ss) [bir_state_set_failed_def]
+) >>
+IMP_RES_TAC bir_exec_step_state_valid_THM >>
+REV_FULL_SIMP_TAC std_ss [] >>
 Cases_on `stmt` >> (
-  ASM_SIMP_TAC std_ss [
-    bir_exec_stmtE_valid_state_invar_cjmp,
-    bir_exec_stmtE_valid_state_invar_jmp,
-    bir_exec_stmtE_valid_state_invar_halt]
+  ASM_SIMP_TAC std_ss [bir_exec_stmt_state_REWRS, bir_exec_stmtE_valid_pc, LET_DEF]
+) >>
+rename1 `bir_exec_stmtB_state stmt st` >>
+Q.ABBREV_TAC `st' = bir_exec_stmtB_state stmt st` >>
+`st'.bst_pc = st.bst_pc` by METIS_TAC[bir_exec_stmtB_pc_unchanged] >>
+COND_CASES_TAC >> ASM_SIMP_TAC (std_ss++bir_TYPES_ss) [bir_pc_next_valid]);
+
+
+val bir_exec_step_well_typed_env = store_thm ("bir_exec_step_well_typed_env",
+``!p st. bir_is_well_typed_env st.bst_environ ==>
+         bir_is_well_typed_env (bir_exec_step_state p st).bst_environ``,
+
+REPEAT STRIP_TAC >>
+ASM_SIMP_TAC (std_ss++boolSimps.LIFT_COND_ss) [bir_exec_step_state_def, bir_exec_step_def] >>
+CASE_TAC >> (
+  ASM_SIMP_TAC (std_ss++bir_TYPES_ss) [bir_state_set_failed_def]
+) >>
+DISJ2_TAC >>
+rename1 `_ = SOME stmt` >>
+Cases_on `stmt` >> (
+  ASM_SIMP_TAC std_ss [GSYM bir_exec_stmt_state_def, bir_exec_stmt_state_REWRS, LET_DEF,
+    bir_exec_stmtE_env_unchanged]
+) >>
+CASE_TAC >> (
+  ASM_SIMP_TAC (std_ss++bir_TYPES_ss) [bir_exec_stmtB_well_typed_env]
 ));
 
 
@@ -391,21 +466,8 @@ val bir_exec_step_valid_state_invar = store_thm ("bir_exec_step_valid_state_inva
 ``!p st. bir_is_valid_state p st ==>
          bir_is_valid_state p (bir_exec_step_state p st)``,
 
-REPEAT STRIP_TAC >>
-IMP_RES_TAC bir_exec_step_state_valid_THM >>
-Cases_on `bir_state_is_terminated st` >> FULL_SIMP_TAC std_ss [] >>
-Cases_on `stmt` >> (
-  ASM_SIMP_TAC std_ss [bir_exec_stmt_state_REWRS, bir_exec_stmtE_valid_state_invar, LET_DEF]
-) >>
-rename1 `bir_exec_stmtB_state stmt st` >>
-Q.ABBREV_TAC `st' = bir_exec_stmtB_state stmt st` >>
-`bir_is_valid_state p st'` by METIS_TAC[bir_exec_stmtB_valid_state_invar] >>
-COND_CASES_TAC >> ASM_SIMP_TAC std_ss [] >>
-`st'.bst_pc = st.bst_pc` by METIS_TAC[bir_exec_stmtB_pc_unchanged] >>
-FULL_SIMP_TAC (arith_ss++holBACore_ss) [bir_is_valid_state_def,
-  bir_get_current_statement_SOME_B, bir_is_valid_pc_def, bir_pc_next_def] >>
-REPEAT BasicProvers.VAR_EQ_TAC >>
-FULL_SIMP_TAC arith_ss []);
+SIMP_TAC std_ss [bir_is_valid_state_def,
+  bir_exec_step_well_typed_env, bir_exec_step_valid_pc]);
 
 
 val _ = export_theory();
